revised NonceST to use monotone, injective maps

src/tls/ConnInvariant.fst
@@ -1,9 +1,12 @@
 module ConnInvariant
 open TLSConstants
 
-module Mm = MonotoneMap
-module Mr = FStar.Monotonic.RRef
-module Hh = FStar.HyperHeap
+
+module MM = MonotoneMap
+module MR = FStar.Monotonic.RRef
+module HH = FStar.HyperHeap
+module MS = MasterSecret
+
 open TLSInfo
 open Handshake
 open Connection
@@ -11,66 +14,66 @@ open Connection
 type id = StreamAE.id
 let r_conn (r:random) = c:connection{c.hs.id = r}
 
-let pairwise_disjoint (m:Mm.map' random r_conn) = 
-    forall r1 r2. r1<>r2 /\ is_Some (Mm.sel m r1) /\ is_Some (Mm.sel m r2)
-	     ==> Hh.disjoint (Some.v (Mm.sel m r1)).region  
-		             (Some.v (Mm.sel m r2)).region
+let pairwise_disjoint (m:MM.map' random r_conn) = 
+    forall r1 r2. r1<>r2 /\ is_Some (MM.sel m r1) /\ is_Some (MM.sel m r2)
+	     ==> HH.disjoint (Some.v (MM.sel m r1)).region  
+		             (Some.v (MM.sel m r2)).region
 
-module Ms = MasterSecret
-let tls_region = Ms.tls_region
 
-type conn_table_t = Mm.t tls_region random r_conn pairwise_disjoint
+let tls_region = MS.tls_region
+
+type conn_table_t = MM.t tls_region random r_conn pairwise_disjoint
 
 let conn_table : conn_table_t = 
-  Mm.alloc #tls_region #random #r_conn #pairwise_disjoint
+  MM.alloc #tls_region #random #r_conn #pairwise_disjoint
 
-type ms_tab = Mm.map' Ms.ids Ms.writer 
-type c_tab  = Mm.map' random r_conn 
+type ms_tab = MM.map' MS.ids MS.writer 
+type c_tab  = MM.map' random r_conn 
 
 assume val idNonce : id -> Tot random
 
-let registered (i:id{StAE.is_stream_ae i}) (w:StreamAE.writer i) (c:connection) (h:Hh.t) = 
-  Hh.disjoint (HS.region c.hs) tls_region /\
-  Hh.contains_ref (HS.log c.hs) h /\
-  (exists e. SeqProperties.mem e  (Hh.sel h (HS.log c.hs)) /\
+let registered (i:id{StAE.is_stream_ae i}) (w:StreamAE.writer i) (c:connection) (h:HH.t) = 
+  HH.disjoint (HS.region c.hs) tls_region /\
+  HH.contains_ref (HS.log c.hs) h /\
+  (exists e. SeqProperties.mem e  (HH.sel h (HS.log c.hs)) /\
       (let i' = Handshake.hsId (Handshake.Epoch.h e) in
         i=i' /\ StAE.stream_ae #i e.w == w))
 
 let ms_conn_invariant (ms:ms_tab)
  		      (conn:c_tab)
 		      (h:HyperHeap.t) 
-  = forall (i:id) (r:Hh.rid).{:pattern (MM.sel ms (i,r))}
+  = forall (i:id) (r:HH.rid).{:pattern (MM.sel ms (i,r))}
 	     authId i /\ StAE.is_stream_ae i ==>  //Focused only on TLS-1.3 for now, hence the is_stream_ae guard
 	            (match MM.sel ms (i,r) with 
 		     | None -> True
 		     | Some w -> 
 		       Map.contains h (StreamAE.State.region w) /\ //technical for framing; need to know that the writer's region exists
- 		       (Mr.m_sel h (StreamAE.ilog (StreamAE.State.log w)) = Seq.createEmpty  \/   //the writer is still unused; or
-		        (let copt = Mm.sel conn (idNonce i) in
+ 		       (MR.m_sel h (StreamAE.ilog (StreamAE.State.log w)) = Seq.createEmpty  \/   //the writer is still unused; or
+		        (let copt = MM.sel conn (idNonce i) in
   			 is_Some copt /\ registered i w (Some.v copt) h)))      //it's been assigned to a connection
 
-let mc_inv (h:HyperHeap.t) = ms_conn_invariant (Mr.m_sel h Ms.ms_tab) (Mr.m_sel h conn_table) h
+let mc_inv (h:HyperHeap.t) = ms_conn_invariant (MR.m_sel h MS.ms_tab) (MR.m_sel h conn_table) h
 
 //Checking the stability of the invariant
 
 //1. Deriving a new key involves adding a new writer to the ms table (because we tried a lookup at id and it failed)
 //   Easy: because a new log is empty and both cases of the conn table allow empty logs to be in ms
-
-val ms_derive_is_ok: h0:HyperHeap.t -> h1:HyperHeap.t -> i:id -> r:Hh.rid -> w:Ms.writer (i,r) 
+ 
+val ms_derive_is_ok: h0:HyperHeap.t -> h1:HyperHeap.t -> i:id -> r:HH.rid -> w:MS.writer (i,r) 
   -> Lemma (requires 
-		 Hh.contains_ref (Mr.as_rref conn_table) h0 /\
-		 Hh.contains_ref (Mr.as_rref Ms.ms_tab) h0 /\
+		 HH.contains_ref (MR.as_rref conn_table) h0 /\
+		 HH.contains_ref (MR.as_rref MS.ms_tab) h0 /\
 		 Map.contains h1 (StreamAE.State.region w) /\
 		 authId i /\ 
 		 StAE.is_stream_ae i /\
 		 mc_inv h0 /\ //we're initially in the invariant
-		 Hh.modifies (Set.singleton tls_region) h0 h1 /\ //we just changed the tls_region
-		 Hh.modifies_rref tls_region !{Hh.as_ref (Mr.as_rref Ms.ms_tab)} h0 h1 /\ //and within it, at most the ms_tab
-		 (let old_ms = Mr.m_sel h0 Ms.ms_tab in 
-		  let new_ms = Mr.m_sel h1 Ms.ms_tab in
-		  Mm.sel old_ms (i,r) = None /\
-		  new_ms = Mm.upd old_ms (i,r) w) /\                                    //and the ms_tab only changed by adding w
-		 Mr.m_sel h1 (StreamAE.ilog (StreamAE.State.log w)) = Seq.createEmpty)             //and w's log is empty
+		 HH.modifies (Set.singleton tls_region) h0 h1 /\ //we just changed the tls_region
+		 HH.modifies_rref tls_region !{HH.as_ref (MR.as_rref MS.ms_tab)} h0 h1 /\ //and within it, at most the ms_tab
+		 (let old_ms = MR.m_sel h0 MS.ms_tab in 
+		  let new_ms = MR.m_sel h1 MS.ms_tab in
+		  MM.sel old_ms (i,r) = None /\
+		  new_ms = MM.upd old_ms (i,r) w) /\                                    //and the ms_tab only changed by adding w
+		 MR.m_sel h1 (StreamAE.ilog (StreamAE.State.log w)) = Seq.createEmpty)             //and w's log is empty
 	 (ensures mc_inv h1)                                                       //we're back in the invariant
 let ms_derive_is_ok h0 h1 i r w = ()
 
@@ -81,39 +84,39 @@ let ms_derive_is_ok h0 h1 i r w = ()
 val add_epoch_ok: h0:HyperHeap.t -> h1:HyperHeap.t -> i:id{StAE.is_stream_ae i /\ authId i} 
 		-> c:r_conn (idNonce i) -> e:epoch (HS.region c.hs) (HS.peer c.hs) 
   -> Lemma (requires 
-            (let ctab = Mr.m_sel h0 conn_table in
-	     let mstab = Mr.m_sel h0 Ms.ms_tab in
+            (let ctab = MR.m_sel h0 conn_table in
+	     let mstab = MR.m_sel h0 MS.ms_tab in
 	     let old_hs_log = HH.sel h0 (HS.log c.hs) in
      	     let new_hs_log = HH.sel h1 (HS.log c.hs) in 
 	     let rgn = HS.region c.hs in
-	     Hh.contains_ref (Mr.as_rref conn_table) h0 /\
-	     Hh.contains_ref (Mr.as_rref Ms.ms_tab) h0 /\
-	     Hh.disjoint (HS.region c.hs) tls_region /\
-	     Hh.contains_ref (HS.log c.hs) h0 /\
-	     Hh.contains_ref (HS.log c.hs) h1 /\
+	     HH.contains_ref (MR.as_rref conn_table) h0 /\
+	     HH.contains_ref (MR.as_rref MS.ms_tab) h0 /\
+	     HH.disjoint (HS.region c.hs) tls_region /\
+	     HH.contains_ref (HS.log c.hs) h0 /\
+	     HH.contains_ref (HS.log c.hs) h1 /\
 	     mc_inv h0 /\ //we're initially in the invariant
 	     i=hsId (Epoch.h e) /\ //the epoch has id it
 	     (let w = StAE.stream_ae #i (Epoch.w e) in //the epoch writer
-	      let epochs = Hh.sel h0 (HS.log c.hs) in
+	      let epochs = HH.sel h0 (HS.log c.hs) in
       	      Map.contains h1 (StreamAE.State.region w) /\
 	      (forall e. SeqProperties.mem e epochs ==> hsId (Epoch.h e) <> i) /\ //i is fresh for c
- 	      Mm.sel mstab (i, rgn) = Some w /\ //we found the writer in the ms_tab
+ 	      MM.sel mstab (i, rgn) = Some w /\ //we found the writer in the ms_tab
 	      MM.sel ctab (idNonce i) = Some c /\ //we found the connection in the conn_table
-	      Hh.modifies_one (HS.region c.hs) h0 h1 /\ //we just modified this connection's handshake region
-	      Hh.modifies_rref (HS.region c.hs) !{Hh.as_ref (HS.log c.hs)} h0 h1 /\ //and within it, just the epochs log
+	      HH.modifies_one (HS.region c.hs) h0 h1 /\ //we just modified this connection's handshake region
+	      HH.modifies_rref (HS.region c.hs) !{HH.as_ref (HS.log c.hs)} h0 h1 /\ //and within it, just the epochs log
 	      new_hs_log = SeqProperties.snoc old_hs_log e))) //and we modified it by adding this epoch to it
 	  (ensures mc_inv h1) //we're back in the invariant
 
 #reset-options "--z3timeout 10 --initial_fuel 2 --max_fuel 2 --initial_ifuel 2 --max_ifuel 2"
 
 let add_epoch_ok h0 h1 i c e = 
-  assert (Mr.m_sel h0 Ms.ms_tab = Mr.m_sel h1 Ms.ms_tab);
-  assert (Mr.m_sel h0 conn_table = Mr.m_sel h1 conn_table);
+  assert (MR.m_sel h0 MS.ms_tab = MR.m_sel h1 MS.ms_tab);
+  assert (MR.m_sel h0 conn_table = MR.m_sel h1 conn_table);
   let w = StAE.stream_ae #i (Epoch.w e) in //the epoch writer
-  assert (Mr.m_sel h0 (StreamAE.ilog (StreamAE.State.log w)) = Mr.m_sel h1 (StreamAE.ilog (StreamAE.State.log w)));
-  let ctab = Mr.m_sel h0 conn_table in
-  let mstab = Mr.m_sel h0 Ms.ms_tab in
-  let copt = Mm.sel ctab (idNonce i) in
+  assert (MR.m_sel h0 (StreamAE.ilog (StreamAE.State.log w)) = MR.m_sel h1 (StreamAE.ilog (StreamAE.State.log w)));
+  let ctab = MR.m_sel h0 conn_table in
+  let mstab = MR.m_sel h0 MS.ms_tab in
+  let copt = MM.sel ctab (idNonce i) in
   let old_hs_log = HH.sel h0 (HS.log c.hs) in
   assert (is_Some copt);
   assert (~ (registered i w (Some.v copt) h0));
@@ -124,12 +127,12 @@ let add_epoch_ok h0 h1 i c e =
   assume (StAE.is_stream_ae j);
   assume (authId j);
   assume (s <> HS.region c.hs);
-  match Mm.sel mstab (j, s) with 
+  match MM.sel mstab (j, s) with 
   | None -> admit()
   | Some wj -> 
     assume (StreamAE.State.region wj <> HS.region c.hs); //can see here why the post-condition fails ... need better separation invariants between the HS.log and the writer logs
-    assume (HH.contains_ref (Mr.as_rref (StreamAE.ilog (StreamAE.State.log wj))) h0);
-    assert (Mr.m_sel h0 (StreamAE.ilog (StreamAE.State.log wj)) = Mr.m_sel h1 (StreamAE.ilog (StreamAE.State.log wj)));
+    assume (HH.contains_ref (MR.as_rref (StreamAE.ilog (StreamAE.State.log wj))) h0);
+    assert (MR.m_sel h0 (StreamAE.ilog (StreamAE.State.log wj)) = MR.m_sel h1 (StreamAE.ilog (StreamAE.State.log wj)));
     admit()
 
 
