src/tls/NonceST.fst
@@ -1,71 +1,87 @@
-﻿module Nonce
-
+﻿module NonceST
 open TLSConstants
-open FStar.Seq
 open Platform.Bytes
 open Platform.Error
 
-open Heap
-open FStar.HyperHeap
+module HH = FStar.HyperHeap
+module MM = MonotoneMap
+module MR = FStar.Monotonic.RRef
 
-type hh = HyperHeap.t
 type random = lbytes 32
-type rid = r:rid{r<>root}
-assume val nonces_region : r:rid{parent r = root}
- 
+
 let ideal = IdealFlags.ideal_Nonce // controls idealization of random sample: collision-avoidance.
 
 val timestamp: unit -> ST (lbytes 4)
   (requires (fun h0 -> True))
   (ensures (fun h0 _ h1 -> modifies Set.empty h0 h1))
- 
 let timestamp () = 
   let time = Platform.Date.secondsFromDawn () in
   lemma_repr_bytes_values time;
   bytes_of_int 4 time
   
-//This workaround doesn't work
-//let op_Colon_Equals (#a:Type) (#i:rid) (r:rref i a) (v:a) = op_Colon_Equals #a #i r v
+// MM.map provide a dependent map type; 
+// In this case, we don't need the dependencey
+// The n_rid type is rid with a trivial depdendence on (n:random)
+let n_rid = fun (n:random) -> rid
 
-type nonce_entry = (r:role * random * rid)
-//let nonce_log = if ideal then rref nonces_region (list nonce_entry) else unit
-//let log = if ideal then ST.alloc #(list nonce_entry) [] else ()
-let log : (rref nonces_region (list nonce_entry)) = ralloc #(list nonce_entry) nonces_region []
+// A partial map from nonces to rid is injective, 
+// if it maps distinct nonces to distinct rids
+let injective (n:MM.map' random n_rid) = 
+  forall n1 n2. n1<>n2 ==> (match MM.sel n n1, MM.sel n n2 with
+			  | Some r1, Some r2 -> r1 <> r2
+			  | _ -> True)
 
-val mkHelloRandom: r:role -> region:rid -> ST random
-  (requires (fun h -> True))
+//nonce_rid_table:
+//  A monotone, injective partial map in the tls_tables_region, from random to rid
+//  Essentially: m:(r:random  -> Tot (n_rid r)) {injective m}
+//  Equivalently m:(random  -> Tot rid) {injective m}
+//We could conditionally allocate this table based on the ideal flag
+//See the style, e.g., in StreamAE
+//However, in this case, we have just a single global table and the additional
+//allocation seems rather mild. Still, would be nice to do remove this allocation someday.
+let nonce_rid_table : MM.t tls_tables_region random n_rid injective =  
+  MM.alloc #tls_tables_region #random #n_rid #injective
+
+//A nonce n is fresh in h if the nonce_rid_table doesn't contain it
+let fresh (n:random) (h:HH.t) = MM.sel (MR.m_sel h nonce_rid_table) n = None
+
+//A region is fresh if no nonce is associated with it
+let fresh_region (r:rid) (h:HH.t) = 
+  forall n. MM.sel (MR.m_sel h nonce_rid_table) n <> Some r
+
+//A nonce n is registered to region r, if the table contains n -> Some r; 
+//This mapping is stable (that's what the MR.witnessed means)
+let registered (n:random) (r:rid) = MR.witnessed (MM.contains nonce_rid_table n r)
+
+//Although the table only maps nonces to rids, externally, we also 
+//want to associate the nonce with a role. Within this module
+//what counts is the stable association of nonce to rid
+//So, we define role_nonce as an abstract predicate to capture the 
+//"event" that mkHelloRandom was called for particular triple of values
+abstract let role_nonce (cs:role) (n:random) (r:rid) = registered n r
+
+val mkHelloRandom: cs:role -> r:rid -> ST random
+  (requires (fun h -> fresh_region r h))
   (ensures (fun h0 n h1 -> 
-    modifies (Set.singleton nonces_region) h0 h1 /\ 
-    modifies_rref nonces_region !{ as_ref log } h0 h1 /\
-    (ideal ==> ~(List.Tot.existsb (fun (r0, n0, _) -> r=r0 && n0=n) (sel h0 log)) /\
-             sel h1 log = (r, n, region) :: sel h0 log )))
-
-let rec mkHelloRandom r region =
-  recall log;
+    HH.modifies (Set.singleton tls_tables_region) h0 h1 /\ //modifies at most the tables region
+    HH.modifies_rref tls_tables_region !{ HH.as_ref (MR.as_rref nonce_rid_table) } h0 h1 /\ //and within it, at most the nonce_rid_tabe
+    (ideal ==> fresh n h0  /\        //if we're ideal then the nonce is fresh
+    	       registered n r /\     //the nonce n is associated with r
+    	       role_nonce cs n r))) //and the triple are associated as well, for ever more
+let rec mkHelloRandom cs r =
+  MR.m_recall nonce_rid_table;
   let n : random = timestamp() @| CoreCrypto.random 28 in
   if ideal then 
-    if List.Tot.existsb (fun (r0, n0, _) -> r=r0 && n0=n) !log
-    then mkHelloRandom r region // formally retry to exclude collisions.
-    else (log := (r, n, region) :: !log; n)
+    match MM.lookup nonce_rid_table n with 
+      | None -> MM.extend nonce_rid_table n r; n
+      | Some _ -> mkHelloRandom cs r // formally retry to exclude collisions.
   else n
 
-
-val lookup: role:role -> n:random -> ST (option rid)
+val lookup: cs:role -> n:random -> ST (option rid)
   (requires (fun h -> True))
-  (ensures (fun h0 rid h1 -> modifies Set.empty h0 h1))
-
-let lookup role n =
-  let entry = List.Tot.tryFind (fun (r0, n0, _) -> role=r0 && n=n0) !log in
-  match entry with
-  | None -> None
-  | Some (_, _, rid) -> Some rid
-
-(*
-val lookup_lemma: r:role -> n:random -> h:hh ->
-  Lemma (requires True)
-  (ensures 
-    let rid = lookup r n in
-    is_Some rid ==> List.Tot.mem (role, n, Some.v rid) (sel h0 log))
-
-let lookup_lemma r n h = ()
-*)
+  (ensures (fun h0 ropt h1 -> 
+	        h0=h1 /\ 
+	        (match ropt with
+		 | Some r ->  registered n r /\ role_nonce cs n r
+		 | None -> fresh n h0)))
+let lookup role n = MM.lookup nonce_rid_table n
